Working on disjoint for store

Compat.v
@@ -41,6 +41,14 @@ Module Compat.
     eapply Hcompat. eauto using access.
   Qed.
 
+  Lemma acc_not : forall m m' t ad,
+    compat m m' t ->
+    ~ access m  t ad ->
+    ~ access m' t ad.
+  Proof.
+    intros * ? ? ?. eauto using acc, sym.
+  Qed.
+
   Corollary access_symmetry : forall m m' t ad,
     compat m m' t ->
     access m t ad <-> access m' t ad.
@@ -65,7 +73,8 @@ Module Compat.
 End Compat.
 
 (* changing an inaccessible address does not interfere with access *)
-Lemma access_inaccessible_address : forall m t ad ad' v,
+(* TODO: maybe remove this one. *)
+Lemma access_inaccessible_address1 : forall m t ad ad' v,
   access m t ad ->
   ~ access m t ad' ->
   access (set m ad' v) t ad.
@@ -74,10 +83,51 @@ Proof.
   eauto using Compat.refl, Compat.inaccessible_address, Compat.acc.
 Qed.
 
+Lemma access_inaccessible_address2 : forall m t ad ad' v,
+  ~ access m t ad' ->
+  access (set m ad' v) t ad ->
+  access m t ad.
+Proof.
+  intros * ? ?.
+  eauto using Compat.refl, Compat.sym, Compat.inaccessible_address, Compat.acc.
+Qed.
+
+Lemma access_inaccessible_address3 : forall m t ad ad' v,
+  ~ access m t ad ->
+  ~ access m t ad' ->
+  ~ access (set m ad' v) t ad.
+Proof.
+  intros * Hnacc Hnacc'.
+  eauto using Compat.refl, Compat.inaccessible_address, Compat.acc_not.
+Qed.
+
 Definition disjoint_memory m ths := forall tid1 tid2 ad,
   access m (getTM ths tid1) ad ->
-  access m (getTM ths tid2) ad ->
-  tid1 = tid2.
+  tid1 <> tid2 ->
+  ~ access m (getTM ths tid2) ad.
+
+Theorem disjoint_memory_preservation' : forall m m' ths ths' tid eff,
+  (forall block, eff <> EF_Spawn block) ->
+  disjoint_memory m ths ->
+  m / ths ~~[tid, eff]~~> m' / ths' ->
+  disjoint_memory m' ths'.
+Proof.
+  intros * Hspawn Hdis Hcstep tid1 tid2 ad' Hacc Hneq.
+  inversion Hcstep; subst.
+  - clear Hcstep; inversion H1; subst.
+    + admit.
+    + admit.
+    + admit.
+    + destruct (Nat.eq_dec tid tid1), (Nat.eq_dec tid tid2); subst; eauto;
+      (rewrite (get_set_eq TM_Nil) || rewrite (get_set_neq TM_Nil));
+      (rewrite (get_set_eq TM_Nil) in * || rewrite (get_set_neq TM_Nil) in *);
+      eauto 8 using Step.store_ad_access,
+                    Step.store_access_backwards,
+                    Step.store_does_not_grant_access1,
+                    access_inaccessible_address2,
+                    access_inaccessible_address3.
+  - exfalso. eapply Hspawn. trivial.
+Qed.
 
 Theorem disjoint_memory_preservation : forall m m' ths ths' tid eff,
   disjoint_memory m ths ->
@@ -85,19 +135,16 @@ Theorem disjoint_memory_preservation : forall m m' ths ths' tid eff,
   disjoint_memory m' ths'.
 Proof.
   intros * Hdis Hcstep tid1 tid2 ad Hacc1 Hacc2.
-  specialize (Hdis tid1 tid2 ad).
+  specialize (Hdis tid1 tid2 ad) as Hdis'.
   inversion Hcstep; subst.
   - clear Hcstep; inversion H1; subst.
     + destruct (Nat.eq_dec tid tid1) as [? | Hneq]; 
       destruct (Nat.eq_dec tid tid2);
       subst; trivial.
-      * exfalso.
-        rewrite (get_set_eq TM_Nil) in Hacc1;
+      * rewrite (get_set_eq TM_Nil) in Hacc1;
         rewrite (get_set_neq TM_Nil) in Hacc2;
         eauto using mstep_none_does_not_grant_access.
-      * exfalso.
-        eapply not_eq_sym in Hneq.
-        rewrite (get_set_eq TM_Nil) in Hacc2;
+      * rewrite (get_set_eq TM_Nil) in Hacc2;
         rewrite (get_set_neq TM_Nil) in Hacc1;
         eauto using mstep_none_does_not_grant_access.
       * rewrite (get_set_neq TM_Nil) in *; eauto.
@@ -105,29 +152,25 @@ Proof.
     + destruct (Nat.eq_dec tid tid1) as [? | Hneq]; 
       destruct (Nat.eq_dec tid tid2);
       subst; trivial.
-      * exfalso.
-        rewrite (get_set_eq TM_Nil) in Hacc1;
+      * rewrite (get_set_eq TM_Nil) in Hacc1;
         rewrite (get_set_neq TM_Nil) in Hacc2;
         eauto using mstep_load_does_not_grant_access.
-      * exfalso.
-        eapply not_eq_sym in Hneq.
-        rewrite (get_set_eq TM_Nil) in Hacc2;
+      * rewrite (get_set_eq TM_Nil) in Hacc2;
         rewrite (get_set_neq TM_Nil) in Hacc1;
         eauto using mstep_load_does_not_grant_access.
       * rewrite (get_set_neq TM_Nil) in *; eauto.
     + destruct (Nat.eq_dec tid tid1) as [? | Hneq]; 
       destruct (Nat.eq_dec tid tid2);
       subst; trivial.
-      * exfalso.
-        rewrite (get_set_eq TM_Nil) in Hacc1;
-        rewrite (get_set_neq TM_Nil) in Hacc2;
-        eauto using mstep_load_does_not_grant_access.
+      * rewrite (get_set_eq TM_Nil) in Hacc1;
+        rewrite (get_set_neq TM_Nil) in Hacc2; eauto.
+        
       * exfalso.
         eapply not_eq_sym in Hneq.
         rewrite (get_set_eq TM_Nil) in Hacc2;
         rewrite (get_set_neq TM_Nil) in Hacc1;
-        eauto using mstep_load_does_not_grant_access.
-      * rewrite (get_set_neq TM_Nil) in *; eauto.
+        eauto using mstep_load_does_not_grant_access. admit.
+      * rewrite (get_set_neq TM_Nil) in *; eauto. admit.
   - admit.
 Qed.
 
